an implementation of cut (not implementable in Rtac)

theories/LambdaWt/SubstWt.v
@@ -8,6 +8,88 @@ Set Implicit Arguments.
 Set Strict Implicit.
 Set Primitive Projections.
 
+Section substI.
+  Variable Tsymbol : Type.
+  Variable TsymbolD : Tsymbol -> Type@{Urefl}.
+  Variable Tsymbol_eq_dec : forall a b : Tsymbol, {a = b} + {a <> b}.
+  Let type := type Tsymbol.
+  Variable Esymbol : type -> Type.
+  Variable EsymbolD : forall t, Esymbol t -> typeD TsymbolD t.
+  Variable Esymbol_eq_dec : forall {t} (a b : Esymbol t), {a = b} + {a <> b}.
+
+  Inductive Unifiable' {tus}
+            (Inst_lookup : forall {ts t}, member (ts,t) tus -> option (wtexpr Esymbol tus ts t))
+            (tvs : list type) (t : type)
+  : wtexpr Esymbol tus tvs t -> wtexpr Esymbol tus tvs t -> Prop :=
+  | Unif_UVar : forall ts (u : member (ts,t) tus) xs e,
+      @Inst_lookup _ _ u = Some e ->
+      @Unifiable' tus Inst_lookup tvs t (wtUVar u xs) (subst xs e).
+
+  Section mid.
+    Variable T : (list (WtExpr.type Tsymbol) * WtExpr.type Tsymbol) -> Type.
+
+    Fixpoint migrator_id' tus {struct tus}
+    : (forall ts t, member (ts,t) tus -> T (ts,t)) ->
+      hlist T tus :=
+      match tus as tus
+            return (forall ts t, member (ts,t) tus -> T (ts,t)) ->
+                   hlist T tus
+      with
+      | nil => fun _ => Hnil
+      | (ts,t) :: tus => fun mk =>
+                           Hcons (@mk _ _ (@MZ _ _ _))
+                                 (migrator_id' (fun ts t z => @mk ts t (MN _ z)))
+      end.
+  End mid.
+
+  Fixpoint vars_id {tus} tvs : hlist (WtExpr.wtexpr Esymbol tus tvs) tvs :=
+    match tvs as tvs
+          return hlist (WtExpr.wtexpr Esymbol tus tvs) tvs
+    with
+    | nil => Hnil
+    | t :: ts =>
+      Hcons (wtVar Esymbol tus (MZ t ts))
+            (hlist_map
+               (fun t' : WtExpr.type Tsymbol => wtexpr_lift (t :: nil) nil)
+               (vars_id ts))
+    end.
+
+  Definition migrator_id tus : migrator Esymbol tus tus :=
+    @migrator_id' _ tus (fun ts t x => wtUVar x (vars_id ts)).
+
+  Definition inst_evolves {tus tus'} (mig : migrator Esymbol tus' tus)
+             (i1 : forall {ts t}, member (ts,t) tus -> option (wtexpr Esymbol tus ts t))
+             (i2 : forall {ts t}, member (ts,t) tus' -> option (wtexpr Esymbol tus' ts t))
+  : Prop :=
+    forall tvs t (e1 e2 : wtexpr Esymbol tus' tvs t),
+      @Unifiable' _ (@i1) _ _ (migrate_expr mig e1) (migrate_expr mig e2) ->
+      @Unifiable' _ (@i2) _ _ e1 e2.
+
+  Class Instantiation (T : list (Tuvar Tsymbol) -> Type) : Type :=
+  { Inst_lookup : forall {tus} (i : T tus) {ts t} (uv : member (ts,t) tus),
+                         option (wtexpr Esymbol tus ts t)
+  ; Inst_set    : forall {tus ts t} (uv : member (ts,t) tus) (e : wtexpr Esymbol tus ts t)
+                         (i : T tus), T tus
+  ; InstD       : forall {tus : list (Tuvar Tsymbol)}
+                         (inst : T tus)
+                         (us : hlist (fun tst =>
+                                        hlist (typeD TsymbolD) (fst tst) -> typeD TsymbolD (snd tst))
+                                     tus), Prop
+  ; Inst_evolves : forall {tus tus'}, migrator Esymbol tus' tus -> T tus -> T tus' -> Prop :=
+      fun tus tus' mig s s' =>
+        inst_evolves mig (@Inst_lookup _ s) (@Inst_lookup _ s')
+  ; Unifiable : forall {tus} (i : T tus) (tvs : list type) (t : type),
+      wtexpr Esymbol tus tvs t -> wtexpr Esymbol tus tvs t -> Prop :=
+      fun tus i => Unifiable' (@Inst_lookup _ i)
+  ; Inst_set_ok : forall tus tvs ts t (u : member (ts,t) tus) w s s',
+      Inst_set u w s = s' ->
+      Inst_lookup s u = None ->
+      inst_evolves (migrator_id _) (@Inst_lookup _ s) (@Inst_lookup _ s') /\
+      forall xs, Unifiable s' (wtUVar u xs) (subst (tvs:=tvs) xs w)
+  }.
+End substI.
+
+
 Section subst.
   Variable Tsymbol : Type.
   Variable TsymbolD : Tsymbol -> Type@{Urefl}.
@@ -25,7 +107,7 @@ Section subst.
   :=
     True.
 
-  Record Inst (tus : list Tuvar) : Type :=
+  Record simple_inst (tus : list Tuvar) : Type :=
   { values   : hlist (fun tst => option (wtexpr tus (fst tst) (snd tst))) tus
   ; _acyclic : Acyclic values }.
 
@@ -35,7 +117,7 @@ Section subst.
                             hlist (typeD TsymbolD) (fst tst) -> typeD TsymbolD (snd tst))
             tus'.
 
-    Fixpoint InstD' (tus : list Tuvar)
+    Fixpoint simple_instD' (tus : list Tuvar)
              (inst : hlist (fun tst => option (wtexpr tus' (fst tst) (snd tst))) tus)
     : hlist (fun tst => hlist (typeD TsymbolD) (fst tst) -> typeD TsymbolD (snd tst))
             tus -> Prop :=
@@ -45,22 +127,22 @@ Section subst.
                          tus -> Prop
       with
       | Hnil => fun _ => True
-      | Hcons None ist => fun us => InstD' ist (hlist_tl us)
+      | Hcons None ist => fun us => simple_instD' ist (hlist_tl us)
       | Hcons (Some val) ist => fun us =>
            (forall cs, hlist_hd us cs = wtexprD EsymbolD val us' cs)
-        /\ InstD' ist (hlist_tl us)
+        /\ simple_instD' ist (hlist_tl us)
       end.
   End instD.
 
-  Definition InstD (tus : list Tuvar)
-             (inst : Inst tus)
+  Definition instD (tus : list Tuvar)
+             (inst : simple_inst tus)
              (us : hlist (fun tst =>
                             hlist (typeD TsymbolD) (fst tst) -> typeD TsymbolD (snd tst))
                          tus)
   : Prop :=
-    @InstD' tus us tus inst.(values) us.
+    @simple_instD' tus us tus inst.(values) us.
 
-  Definition Inst_lookup {tus} (i : Inst tus) {ts t} (uv : member (ts,t) tus)
+  Definition simple_inst_lookup {tus} (i : simple_inst tus) {ts t} (uv : member (ts,t) tus)
   : option (wtexpr tus ts t) :=
     hlist_get uv i.(values).
 
@@ -125,65 +207,35 @@ Section subst.
 
   End hlist_set.
 
-  Definition Inst_set {tus ts t} (uv : member (ts,t) tus) (e : wtexpr tus ts t)
-             (i : Inst tus)
-  : Inst tus :=
+  Definition simple_inst_set {tus ts t} (uv : member (ts,t) tus) (e : wtexpr tus ts t)
+             (i : simple_inst tus)
+  : simple_inst tus :=
     {| values := hlist_set (Some e) uv i.(values)
      ; _acyclic := I
      |}.
 
-  Inductive Unifiable {tus} (s : Inst tus) (tvs : list type) (t : type)
+(*
+  Inductive Unifiable {tus} (s : simple_inst tus) (tvs : list type) (t : type)
   : wtexpr tus tvs t -> wtexpr tus tvs t -> Prop :=
   | Unif_UVar : forall ts (u : member (ts,t) tus) xs e,
       Inst_lookup s u = Some e ->
       @Unifiable tus s tvs t (wtUVar u xs) (subst xs e).
+*)
 
 (*
   Definition Unifiable_eq {tus} s tvs t a b : Prop :=
     @Unifiable tus s tvs t a b \/ @Unifiable tus s tvs t b a.
 *)
 
-  Fixpoint vars_id {tus} tvs : hlist (WtExpr.wtexpr Esymbol tus tvs) tvs :=
-    match tvs as tvs
-          return hlist (WtExpr.wtexpr Esymbol tus tvs) tvs
-    with
-    | nil => Hnil
-    | t :: ts =>
-      Hcons (wtVar Esymbol tus (MZ t ts))
-            (hlist_map
-               (fun t' : WtExpr.type Tsymbol => wtexpr_lift (t :: nil) nil)
-               (vars_id ts))
-    end.
-
-  Section mid.
-    Variable T : (list (WtExpr.type Tsymbol) * WtExpr.type Tsymbol) -> Type.
-
-    Fixpoint migrator_id' tus {struct tus}
-    : (forall ts t, member (ts,t) tus -> T (ts,t)) ->
-      hlist T tus :=
-      match tus as tus
-            return (forall ts t, member (ts,t) tus -> T (ts,t)) ->
-                   hlist T tus
-      with
-      | nil => fun _ => Hnil
-      | (ts,t) :: tus => fun mk =>
-                           Hcons (@mk _ _ (@MZ _ _ _))
-                                 (migrator_id' (fun ts t z => @mk ts t (MN _ z)))
-      end.
-  End mid.
-
-  Definition migrator_id tus : migrator Esymbol tus tus :=
-    @migrator_id' _ tus (fun ts t x => wtUVar x (vars_id ts)).
-
   Lemma hlist_get_migrator_id' : forall T ts t tus mk (m : member (ts,t) tus),
-      hlist_get m (@migrator_id' T tus mk) = mk _ _ m.
+      hlist_get m (@migrator_id' Tsymbol T tus mk) = mk _ _ m.
   Proof.
     induction m; simpl; auto.
     destruct l. simpl. rewrite IHm. reflexivity.
   Qed.
 
   Lemma hlist_get_migrator_id : forall ts t tus (m : member (ts,t) tus),
-      hlist_get m (migrator_id tus) = wtUVar m (vars_id _).
+      hlist_get m (migrator_id Esymbol tus) = wtUVar m (vars_id _ _).
   Proof.
     intros. unfold migrator_id.
     rewrite hlist_get_migrator_id'. reflexivity.
@@ -219,7 +271,7 @@ Section subst.
   Qed.
 
   Theorem migrate_expr_migrate_id : forall tus tvs t (e : wtexpr tus tvs t),
-      migrate_expr (migrator_id _) e = e.
+      migrate_expr (migrator_id _ _) e = e.
   Proof.
     induction e; simpl; intros; auto.
     { rewrite IHe1. rewrite IHe2. reflexivity. }
@@ -239,46 +291,47 @@ Section subst.
                                           Hnil (Hcons Z Hnil)). }
   Qed.
 
+(*
   Definition Inst_evolves {tus tus'} (mig : migrator Esymbol tus' tus)
              (i1 : Inst tus) (i2 : Inst tus') : Prop :=
     forall tvs t (e1 e2 : wtexpr tus' tvs t),
       wtexpr_equiv (Unifiable i1) (migrate_expr mig e1) (migrate_expr mig e2) ->
       wtexpr_equiv (Unifiable i2) e1 e2.
+*)
 
-  Theorem Inst_set_ok : forall tus tvs ts t (u : member (ts,t) tus) w s s',
-      Inst_set u w s = s' ->
-      Inst_lookup s u = None ->
-      Inst_evolves (migrator_id _) s s' /\
-      forall xs, Unifiable s' (wtUVar u xs) (subst (tvs:=tvs) xs w).
+  Theorem simple_inst_set_ok : forall tus tvs ts t (u : member (ts,t) tus) w s s',
+      simple_inst_set u w s = s' ->
+      simple_inst_lookup s u = None ->
+      inst_evolves (migrator_id _ _) (@simple_inst_lookup _ s) (@simple_inst_lookup _ s') /\
+      forall xs, @Unifiable' Tsymbol Esymbol _ (@simple_inst_lookup _ s')
+                            _ _ (wtUVar u xs) (subst (tvs:=tvs) xs w).
   Proof.
     intros. subst.
     split.
     { red. intros.
       do 2 rewrite migrate_expr_migrate_id in H.
-      induction H; try solve [ constructor; eauto ].
-      - constructor.
-        clear - H.
-        induction H; constructor; auto.
-      - constructor.
-        inversion pf. constructor. subst.
-        unfold Inst_lookup, Inst_set. simpl.
-        etransitivity; [ | eapply H ].
-        unfold Inst_lookup.
-        clear - H0 H u0 u Tsymbol_eq_dec.
-        eapply (@hlist_get_set_neq' _ _ _ (Some w) _ _ u0 u (values s)).
-        intros. intro.
-        subst. unfold Inst_lookup in *.
-        inversion pf. subst.
-        rewrite (UIP_refl pf) in H.
-        congruence.
-      - eapply eqTrans; eauto. }
+      destruct H. constructor.
+      unfold simple_inst_lookup, simple_inst_set.
+      simpl.
+      rewrite <- H.
+      eapply (@hlist_get_set_neq' _ _ _ (Some w) _ _ u0 u (values s)).
+      clear - Tsymbol_eq_dec H H0.
+      inversion pf. subst.
+      rewrite (UIP_refl pf).
+      intro. subst. congruence. }
     { intros.
-      constructor. unfold Inst_lookup, Inst_set.
+      constructor. unfold simple_inst_lookup, simple_inst_set.
       simpl. rewrite hlist_get_set. reflexivity. }
     Unshelve.
     eapply pair_eq_dec.
     eapply list_eq_dec. eapply type_eq_dec. eapply Tsymbol_eq_dec.
     eapply type_eq_dec. eapply Tsymbol_eq_dec.
   Defined.
+
+  Global Instance Instantiation_simple_inst : @Instantiation Tsymbol TsymbolD Esymbol simple_inst :=
+  { Inst_lookup := @simple_inst_lookup
+  ; Inst_set    := @simple_inst_set
+  ; InstD       := @instD
+  ; Inst_set_ok := simple_inst_set_ok }.
 
 End subst.
