theories/LambdaWt/WtTactic.v
@@ -16,6 +16,9 @@ Section simple_dep_types.
   Variable EsymbolD : forall t, Esymbol t -> typeD TsymbolD t.
   Variable Esymbol_eq_dec : forall t (a b : Esymbol t), {a = b} + {a <> b}.
 
+  Context (Inst : list _ -> Type)
+          {Inst_Inst : Instantiation TsymbolD Esymbol Inst}.
+
   Section logicT.
     Variable tyProp : type Tsymbol.
     Variable forall_prop : forall (T : Type),
@@ -70,21 +73,48 @@ Section simple_dep_types.
     | wtHyp    : wtexpr Esymbol tus tvs tyProp -> wtgoal tus tvs -> wtgoal tus tvs
     | wtAll    : forall t, wtgoal tus (t :: tvs) -> wtgoal tus tvs.
 
+    Variable tyProp_to_Prop : typeD TsymbolD tyProp -> Prop.
+    Variable Prop_to_tyProp : Prop -> typeD TsymbolD tyProp.
+
+    Fixpoint wtgoalD {tus tvs} (g : wtgoal tus tvs) {struct g}
+    : exprT TsymbolD tus tvs (typeD TsymbolD tyProp) :=
+      match g with
+      | wtSolved _ _ => pure (Prop_to_tyProp True)
+      | wtGoal g => wtexprD EsymbolD g
+      | wtConj l r =>
+        ap (ap
+              (pure (fun x y => Prop_to_tyProp (tyProp_to_Prop x /\ tyProp_to_Prop y)))
+              (wtgoalD l))
+           (wtgoalD r)
+      | wtHyp h g => ap (ap (pure impl_prop) (wtexprD EsymbolD h)) (wtgoalD g)
+      | @wtAll _ _ t g =>
+        let gD := wtgoalD g in
+        ap (T:=exprT TsymbolD tus tvs) (pure (@forall_prop (typeD TsymbolD t)))
+           (fun us vs v => gD us (Hcons v vs))
+      end.
+
     Variables Pre Post : list (Tuvar Tsymbol) -> list (type Tsymbol) -> Type.
+
+    Record resultC tus tvs : Type := mkResultC
+    { resultUs       : _
+    ; result         : Post resultUs tvs
+    ; resultPrems    : list (wtexpr Esymbol resultUs tvs tyProp)
+    ; resultSubst    : Inst resultUs
+    ; resultMigrator : migrator Esymbol tus resultUs }.
+    Arguments mkResultC {_ _} _ _ _ _ _ : clear implicits.
+
+    Definition logicC tus tvs : Type :=
+      forall
+        (prems : list (wtexpr Esymbol tus tvs tyProp))
+        (inst  : Inst tus)
+        (goal  : Pre tus tvs),
+        m (resultC tus tvs).
 
     (** NOTE: [logicT] does not form a monad due to the generalization
      **       over the indices.
      **)
     Definition logicT : Type :=
-      forall tus tvs
-        (prems : list (wtexpr Esymbol tus tvs tyProp))
-        (inst  : Inst Esymbol tus)
-        (goal  : Pre tus tvs),
-        m { tus' : _
-          & Post tus' tvs
-          * list (wtexpr Esymbol tus' tvs tyProp)
-          * Inst Esymbol tus'
-          * migrator Esymbol tus tus' }%type.
+      forall tus tvs, logicC tus tvs.
 
     Variable PreD
     : forall {tus tvs}, Pre tus tvs ->
@@ -94,41 +124,44 @@ Section simple_dep_types.
                         exprT TsymbolD tus tvs (typeD TsymbolD tyProp).
     Variable mD : forall T (TD : T -> Prop), m T -> Prop.
 
-    Variable tyProp_to_Prop : typeD TsymbolD tyProp -> Prop.
-    Variable Prop_to_tyProp : Prop -> typeD TsymbolD tyProp.
-
-    Definition logicT_spec (l : logicT) : Prop :=
-      forall tus tvs prems goal inst result,
-        l tus tvs prems inst goal = result ->
+    Definition logicC_spec {tus tvs} (c : logicC tus tvs) : Prop :=
+      forall prems goal inst result,
+        c prems inst goal = result ->
         mD (fun t =>
-                let '(existT _ tus' (post, prems', inst', trans)) := t in
+                match t with
+                | mkResultC tus' post prems' inst' trans =>
                 Inst_evolves trans inst' inst /\
                 @foralls_uvar_prop tus' (fun us' =>
                   let us := migrate_env EsymbolD trans us' in
-                  InstD EsymbolD inst' us' ->
+                  InstD inst' us' ->
                   tyProp_to_Prop
                     (@foralls_prop tvs (fun vs =>
                        impl_prop (impls_prop (map (fun p => wtexprD EsymbolD p us' vs) prems')
                                              (@PostD _ _ post us' vs))
                                  (impls_prop (map (fun p => wtexprD EsymbolD p us vs) prems)
-                                             (@PreD  _ _ goal us  vs))))))
+                                             (@PreD  _ _ goal us  vs)))))
+                end)
            result.
+
+    Definition logicT_spec (l : logicT) : Prop :=
+      forall tus tvs,
+        logicC_spec (l tus tvs).
   End logicT.
 
   Require Import MirrorCore.LambdaWt.Unify.
+  Require Import ExtLib.Structures.Monads.
+  Require Import ExtLib.Structures.Functor.
 
   Section assumption_tactic.
     Variable tyProp : type Tsymbol.
     Variable m : Type -> Type.
-    Require Import ExtLib.Structures.Monads.
-    Require Import ExtLib.Structures.Functor.
     Context {Monad_m : Monad m}.
     Context {MonadPlus_m : MonadPlus m}.
     Context {MonadZero_m : MonadZero m}.
     Context {Functor_m : Functor m}.
 
-    Variable unify : Unifier Esymbol (Inst Esymbol).
-    Variable unifyOk : UnifierOk (@Inst_lookup _ Esymbol) unify.
+    Variable unify : Unifier Esymbol Inst.
+    Variable unifyOk : UnifierOk unify.
 
     Variable mD : forall T (TD : T -> Prop), m T -> Prop.
     Variable forall_prop : forall (T : Type),
@@ -182,11 +215,11 @@ Section simple_dep_types.
       Context {tus : list (Tuvar Tsymbol)}.
       Context {tvs : list (type Tsymbol)}.
       Variables (gl : wtexpr Esymbol tus tvs tyProp)
-                (s : Inst Esymbol tus).
+                (s : Inst tus).
 
       Fixpoint find_premise
                (prems : list (wtexpr Esymbol tus tvs tyProp))
-      : m (Inst Esymbol tus) :=
+      : m (Inst tus) :=
         match prems with
         | nil => mzero
         | p :: ps =>
@@ -199,7 +232,7 @@ Section simple_dep_types.
 
       Local Lemma find_premise_sound
       : forall prems,
-          mD (fun inst' : Inst Esymbol tus =>
+          mD (fun inst' : Inst tus =>
                 let trans := migrator_id Esymbol tus in
                 SubstWt.Inst_evolves trans inst' s /\
                 foralls_uvar_prop
@@ -208,7 +241,7 @@ Section simple_dep_types.
                              (fun tst : list (type Tsymbol) * type Tsymbol =>
                                 hlist (typeD TsymbolD) (fst tst) -> typeD TsymbolD (snd tst))
                              tus =>
-                      InstD EsymbolD inst' us ->
+                      InstD inst' us ->
                       tyProp_to_Prop
                         (foralls_prop tyProp forall_prop
                                       (fun vs : hlist (typeD TsymbolD) tvs =>
@@ -242,16 +275,16 @@ Section simple_dep_types.
              (fun _ _ => unit) :=
       fun tus tvs prems sub goal =>
         fmap (F:=m)
-             (fun sub' => @existT _ _ tus (tt,prems,sub',migrator_id _ _))
+             (fun sub' => mkResultC (fun _ _ => unit) tt prems sub' (migrator_id _ _))
              (find_premise goal sub prems).
 
     Theorem Assumption_sound
-    : logicT_spec forall_prop impl_prop
+    : logicT_spec forall_prop impl_prop tyProp_to_Prop
                   (fun tus tvs e => wtexprD EsymbolD e)
                   (fun _ _ _ => Pure_exprT (Prop_to_tyProp True))
-                  mD tyProp_to_Prop Assumption.
+                  mD Assumption.
     Proof.
-      red. unfold Assumption. intros.
+      red. red. unfold Assumption. intros.
       subst.
       eapply mD_fmap
       with (Q:=fun inst' =>
@@ -263,7 +296,7 @@ Section simple_dep_types.
                               (fun tst : list (type Tsymbol) * type Tsymbol =>
                                  hlist (typeD TsymbolD) (fst tst) ->
                                  typeD TsymbolD (snd tst)) tus =>
-                       InstD EsymbolD inst' us ->
+                       InstD inst' us ->
                        tyProp_to_Prop
                          (foralls_prop tyProp forall_prop
                                        (fun vs : hlist (typeD TsymbolD) tvs =>
@@ -278,6 +311,85 @@ Section simple_dep_types.
       eapply find_premise_sound.
     Admitted.
   End assumption_tactic.
+
+  Section cut_tactic.
+    Variable tyProp : type Tsymbol.
+    Variable m : Type -> Type.
+    Context {Monad_m : Monad m}.
+    Context {MonadPlus_m : MonadPlus m}.
+    Context {MonadZero_m : MonadZero m}.
+    Context {Functor_m : Functor m}.
+
+    Variable unify : Unifier Esymbol Inst.
+    Variable unifyOk : UnifierOk unify.
+
+    Variable mD : forall T (TD : T -> Prop), m T -> Prop.
+    Variable forall_prop : forall (T : Type),
+        (T -> typeD TsymbolD tyProp) ->
+        typeD TsymbolD tyProp.
+    Variable impl_prop :
+        typeD TsymbolD tyProp ->
+        typeD TsymbolD tyProp ->
+        typeD TsymbolD tyProp.
+
+    Variable tyProp_to_Prop : typeD TsymbolD tyProp -> Prop.
+    Variable Prop_to_tyProp : Prop -> typeD TsymbolD tyProp.
+
+    Hypothesis mD_mzero : forall T (P : T -> _), mD P mzero.
+    Hypothesis mD_fmap : forall T U (f : T -> U) (P Q : _ -> Prop) x,
+        (forall x, Q x -> P (f x)) ->
+        mD Q x ->
+        mD P (fmap f x).
+    Hypothesis mD_mplus : forall T U (P : T -> Prop) (Q : U -> Prop)
+                                 (x : m T) (y : m U),
+        mD P x ->
+        mD Q y ->
+        mD (fun x => match x with
+                     | inl x => P x
+                     | inr x => Q x
+                     end) (mplus x y).
+    Hypothesis mD_bind : forall T U (P : T -> Prop) (Q : U -> Prop) c k,
+        mD P c ->
+        (forall x, P x -> mD Q (k x)) ->
+        mD Q (bind c k).
+    Hypothesis mD_ret : forall T (P : T -> Prop) x,
+        P x -> mD P (ret x).
+
+    Hypothesis mD_conseq : forall T (P Q : T -> Prop) x,
+        mD Q x ->
+        (forall x, Q x -> P x) ->
+        mD P x.
+
+    Definition Cut {tus tvs} (t : wtexpr Esymbol tus tvs tyProp)
+    : logicC tyProp m
+             (fun tus tvs => wtexpr Esymbol tus tvs tyProp)
+             (fun tus tvs => wtgoal tyProp tus tvs)%type
+             tus tvs :=
+      fun prems sub goal =>
+        ret (m:=m) (mkResultC (wtgoal tyProp)
+                              (wtConj (wtGoal t) (wtHyp t (wtGoal goal)))
+                              prems
+                              sub
+                              (migrator_id _ _)).
+
+
+    Existing Instance Reflexive_Inst_evolves.
+
+    Theorem Cut_sound
+    : forall tus tvs t,
+        logicC_spec forall_prop impl_prop tyProp_to_Prop
+                    (fun tus tvs e => wtexprD EsymbolD e)
+                    (fun _ _ e => @wtgoalD tyProp forall_prop impl_prop tyProp_to_Prop Prop_to_tyProp _ _ e)
+                    mD
+                    (@Cut tus tvs t).
+    Proof.
+      unfold Cut. red. simpl; intros. subst.
+      eapply mD_ret.
+      split; [ reflexivity | ].
+      { simpl. admit. }
+    Admitted.
+
+  End cut_tactic.
 
 End simple_dep_types.
 
